nola/examples/rust_halt/box.v
@@ -22,8 +22,8 @@ Section ty_box.
   (** [ty_box] is productive *)
   #[export] Instance ty_box_productive {X} : Productive (@ty_box X).
   Proof.
-    move=> ?[??][??] /ty_proeq_later [/=eqO eqS].
-    rewrite ty_box_unseal /ty_box_def. apply ty_proeq=>/=. split=> >.
+    move=> ?[??][??] /ty_proeqv_later [/=eqO eqS].
+    rewrite ty_box_unseal /ty_box_def. apply ty_proeqv=>/=. split=> >.
     { do 4 f_equiv=> ?. by rewrite eqO. } { do 3 f_equiv=> ?. by rewrite eqS. }
   Qed.
   #[export] Instance ty_box_proper {X} : Proper ((≡) ==> (≡)) (@ty_box X).
